Fix/SumETheories.v
@@ -1,0 +1,137 @@
+Set Implicit Arguments.
+Set Maximal Implicit Insertion.
+Set Contextual Implicit.
+
+Require Import GHC.Base.
+
+Require Import Fix.Fix.
+Require Import Fix.SumE.
+
+From Coq Require Import
+  Relation_Definitions
+  RelationClasses
+  FinFun
+.
+
+(** * Theories for ⊕ *)
+
+Definition commMapping {F G : (Set -> Set) -> Set -> Set}
+  {E : Set -> Set} {R : Set} (a : (F ⊕ G) E R) : (G ⊕ F) E R :=
+  match a with
+  | Inl1 f => Inr1 f
+  | Inr1 g => Inl1 g
+  end.
+
+Lemma Bijective__commMapping :
+  forall {F G : (Set -> Set) -> Set -> Set} {E : Set -> Set} {R : Set},
+    Bijective (@commMapping F G E R).
+Proof.
+  intros. exists commMapping. split.
+  - destruct x; cbn; reflexivity.
+  - destruct y; cbn; reflexivity.
+Qed.
+
+Definition assocMapping {F G H : (Set -> Set) -> Set -> Set}
+  {E : Set -> Set} {R : Set} (a : ((F ⊕ G) ⊕ H) E R) : (F ⊕ (G ⊕ H)) E R :=
+  match a with
+  | Inl1 (Inl1 f) => Inl1 f
+  | Inl1 (Inr1 g) => Inr1 (Inl1 g)
+  | Inr1 h => Inr1 (Inr1 h)
+  end.
+
+Lemma Bijective__assocMapping :
+  forall {F G H : (Set -> Set) -> Set -> Set} {E : Set -> Set} {R : Set},
+    Bijective (@assocMapping F G H E R).
+Proof.
+  intros.
+  exists (fun a => match a with
+           | Inl1 f => Inl1 (Inl1 f)
+           | Inr1 (Inl1 g) => Inl1 (Inr1 g)
+           | Inr1 (Inr1 h) => Inr1 h
+           end).
+  split.
+  - destruct x as [[f | g] | h]; cbn; reflexivity.
+  - destruct y as [f | [g | h]]; cbn; reflexivity.
+Qed.
+
+Definition equiv1 (F G : (Set -> Set) -> Set -> Set) :=
+  forall (E : Set -> Set) (R : Set),
+  exists (f : F E R -> G E R), Bijective f.
+
+Instance Equivalence__equiv1 : Equivalence equiv1.
+Proof.
+  constructor.
+  - intros x E R. exists id. exists id.
+    split; reflexivity.
+  - intros x y Hxy E R.
+    specialize (Hxy E R). destruct Hxy as (f & g & Hf & Hg).
+    exists g. exists f. tauto.
+  - intros x y z Hxy Hyz E R.
+    specialize (Hxy E R). specialize (Hyz E R).
+    destruct Hxy as (f & g & Hf & Hg).
+    destruct Hyz as (h & i & Hh & Hi).
+    exists (h ∘ f). exists (g ∘ i). split; unfold "∘"; intros a.
+    + rewrite Hh. apply Hf.
+    + rewrite Hg. apply Hi.
+Qed.
+
+Notation "x ≈ y" := (equiv1 x y) (at level 43, right associativity).
+
+Theorem comm__Sum1 : forall (F G : (Set -> Set) -> Set -> Set),
+    F ⊕ G ≈ G ⊕ F.
+Proof.
+  intros F G E R. eapply ex_intro. apply Bijective__commMapping.
+Qed.
+
+Theorem assoc__Sum1 : forall (F G H : (Set -> Set) -> Set -> Set),
+    (F ⊕ G) ⊕ H ≈ F ⊕ (G ⊕ H).
+Proof.
+  intros F G H E R. eapply ex_intro. apply Bijective__assocMapping.
+Qed.
+
+(** * Theories for ⊎ *)
+
+Definition equivRel {F : Set -> Set}
+  (P Q : (forall (A : Set), relation (F A)) -> forall (A : Set), relation (F A)) :=
+  forall (K : forall (A : Set), relation (F A)) (A : Set) (a b : F A),
+    P K _ a b <-> Q K _ a b.
+
+Instance Equivalence__equivRel {F : Set -> Set} : Equivalence (@equivRel F).
+Proof.
+  constructor.
+  - intros P K A a b. reflexivity.
+  - intros P Q HPQ K A a b. symmetry. apply HPQ.
+  - intros P Q R HPQ HQR K A a b. etransitivity.
+    + apply HPQ.
+    + apply HQR.
+Qed.
+
+Notation "P ⇔ Q" := (equivRel P Q) (at level 43, right associativity).
+
+Theorem comm__SumRel {F : Set -> Set} :
+  forall (P Q : (forall (A : Set), relation (F A)) -> forall (A : Set), relation (F A)),
+    P ⊎ Q ⇔ Q ⊎ P.
+Proof.
+  intros P Q K A a b. split; destruct 1; (left + right); assumption.
+Qed.
+
+Theorem assoc__SumRel {F : Set -> Set} :
+  forall (P Q R : (forall (A : Set), relation (F A)) -> forall (A : Set), relation (F A)),
+    (P ⊎ Q) ⊎ R ⇔ P ⊎ (Q ⊎ R).
+Proof.
+  intros P Q R K A a b. split; intros.
+  all: repeat match goal with
+       | H : context[?P ⊎ ?Q] |- _ =>
+           destruct H
+         end.
+  all: (left + right); (assumption + left + right); assumption.
+Qed.
+
+Theorem idem__SumRel {F : Set -> Set} :
+  forall (P : (forall (A : Set), relation (F A)) -> forall (A : Set), relation (F A)),
+    P ⇔ P ⊎ P.
+Proof.
+  intros P K A a b. split.
+  - left. assumption.
+  - destruct 1; assumption.
+Qed.
